%%%%%%%PACKAGES%%%%%%%
\documentclass[10pt,twoside,openany]{memoir}


\usepackage[p,osf]{scholax}
% T1 and textcomp are loaded by package. Change that here, if you want
% load sans and typewriter packages here, if needed
\usepackage{amsmath,amsthm}% must be loaded before newtxmath
% amssymb should not be loaded
\usepackage[scaled=1.075,ncf,vvarbb]{newtxmath}% need to scale up math package
% vvarbb selects the STIX version of blackboard bold.


\usepackage{titlesec}
    \titlespacing*{\chapter}
    {0pt} % Left margin
    {*1} % Space before the chapter number (increase this value for more space)
    {0pt} % Space after the chapter number and before the title
\usepackage{anyfontsize}
\usepackage{fancybox}
\usepackage[dvipsnames,svgnames,x11names,hyperref]{xcolor}
\usepackage{enumerate}
\usepackage{comment}
\usepackage{amsfonts}
\usepackage{amsthm}
\usepackage{mathrsfs}
\usepackage{hyperref}
\usepackage{fullpage}
\usepackage{bm}
\usepackage{cprotect}
\usepackage{calligra}
\usepackage{emptypage}
\usepackage{titleps}
\usepackage{microtype}
\usepackage{float}
\usepackage{ocgx}
\usepackage{appendix}
\usepackage{graphicx}
\usepackage{pdfcomment}
\usepackage{enumitem}
\usepackage{mathtools}
\usepackage{tikz-cd}
\usepackage{relsize}
\usepackage[font=footnotesize,labelfont=bf]{caption}
\usepackage{changepage}
\usepackage{xcolor}
\usepackage{ulem}
\usepackage{pgfplots}
\usepackage{marginnote}
    \newcommand*{\mnote}[1]{ % <----------
    \checkoddpage
    \ifoddpage
        \marginparmargin{left}
    \else
        \marginparmargin{right}
    \fi
        \marginnote{\tiny \textcolor{oorange}{#1}}
    }
\usepackage{datetime}
    \newdateformat{specialdate}{\THEYEAR\ \monthname\ \THEDAY}
\usepackage[margin=0.9in]{geometry}
    \setlength{\voffset}{-0.4in}
    \setlength{\headsep}{30pt}
\usepackage{fancyhdr}
    \fancyhf{}
    \cfoot{\footnotesize \thepage}
    \fancyhead[R]{\footnotesize \rightmark}
    \fancyhead[L]{\footnotesize \leftmark}
\usepackage[outline]{contour}% http://ctan.org/pkg/contour
    \renewcommand{\arraystretch}{1.5}
    \contourlength{0.4pt}
    \contournumber{10}%
\usepackage{letterspace}
    \linespread{1.25}
\usepackage{thmtools}
    \declaretheoremstyle[
        spaceabove=6pt, spacebelow=6pt,
        headfont=\normalfont\bfseries,
        notefont=\mdseries, notebraces={(}{)},
        bodyfont=\normalfont,
        postheadspace=1em
        %qed=\qedsymbol
        ]{mystyle}

    \declaretheorem[
        numberwithin=section,
        %shaded={
        %    rulecolor={RGB}{255,250,177},
        %    rulewidth=5pt, 
        %    bgcolor={RGB}{255,250,177}}
    ]{theorem}

    \declaretheorem[
        sibling=theorem,
        numberwithin=section,
        %shaded={
        %    rulecolor=Lavender,
        %    rulewidth=5pt, 
        %    bgcolor=Lavender}
    ]{lemma}

    \declaretheorem[
        sibling=theorem,
        numberwithin=section,
        %shaded={
        %    rulecolor=Lavender,
        %    rulewidth=5pt, 
        %    bgcolor=Lavender}
    ]{proposition}

    \declaretheorem[
        sibling=theorem,
        numberwithin=section,
        %shaded={
        %    rulecolor=Lavender,
        %    rulewidth=5pt, 
        %    bgcolor=Lavender}
    ]{corollary}

    \declaretheorem[
        numberwithin=section,
        style=mystyle,
        %shaded={
        %    rulecolor={RGB}{233,233,233},
        %    rulewidth=5pt, 
        %    bgcolor={RGB}{233,233,233}}
    ]{example}

    \declaretheorem[
        numberwithin=section,
        style=mystyle,
        %shaded={
        %    rulecolor={RGB}{255,250,177},
        %    rulewidth=5pt, 
        %    bgcolor={RGB}{255,250,177}}
    ]{definition}

    \declaretheorem[
        %shaded={
        %    rulecolor=Lavender,
        %    rulewidth=5pt, 
        %    bgcolor=Lavender}
    ]{exercise}
\declaretheorem[numbered=unless unique,style=mystyle]{Note}
    




%%%%%%%%%%%%%%%%%%%%%%
%%%%%%%%MACROS%%%%%%%%
%%%%%%%%%%%%%%%%%%%%%%
\input{/Users/gcrescenzo/Documents/School/LaTeX Documents/Class Notes/makros.tex}




%%%%%%%%%%%%%%%%%%%%%%
%%%%DOCUMENT SETUP%%%%
%%%%%%%%%%%%%%%%%%%%%%
\setsecnumdepth{subsection}
\definecolor{darkgreen}{rgb}{0, 0.5976, 0}
\hypersetup{pdfauthor=Gianluca Crescenzo, pdftitle=Real Analysis I Notes, pdfstartview=FitH, colorlinks=true, linkcolor=darkgreen, citecolor=darkgreen}

\begin{document}
\begin{center}
    { \Large Math 310 \\[0.1in]Homework 5 \\[0.1in]
    Due: 10/9/2024}\\[.25in]
    { Name:} {\underline{Gianluca Crescenzo\hspace*{2in}}}\\[0.15in]
    \end{center}
    \vspace{4pt}
%%%%%%%%%%%%%%%%%%%%%%%%%%%%%%%%%%%%%%%%%%%%%%%%%%%%%%%%%%%%%%%%%%%%%%%%%%%%%%%%%%%%%%%%%%%%%%%%%%%%%%%%%%%%%%%   
    \begin{exercise}
        Let $x_1 = 1$ and inductively set $x_{n+1} = \sqrt{2 +x_n}$. Show that $(x_n)_n$ converges and find its limit.
    \end{exercise}
        \begin{proof}
            Claim: $x_n \leq 2$ for all $n$. We prove this by induction on $n$. Clearly $x_1 = 1 \leq 2$. Now assume our hypothesis is true for $n$. For $n+1$ we have:
                \begin{equation*}
                \begin{split}
                    x_{n+1}
                    & = \sqrt{2 + x_n} \\
                    & \leq \sqrt{2 + 2} \\
                    & = 2.
                \end{split}
                \end{equation*}
            Claim: $x_n \leq x_{n+1}$. Observe that:
                \begin{equation*}
                \begin{split}
                    x_n \leq x_{n+1}
                    & \iff x_n \leq \sqrt{2 + x_n} \\
                    & \iff x_n \leq \sqrt{2 + 2} \\
                    & \iff x_n \leq 2.
                \end{split}
                \end{equation*}
            Since $(x_n)_n$ is increasing and bounded above, by the monotone convergence theorem it has a limit, call it $L$. Thus:
                \begin{equation*}
                \begin{split}
                    \lim_{n \rightarrow \infty}x_{n+1} = \lim_{n \rightarrow \infty}\sqrt{2 + x_n}
                \end{split}
                \end{equation*}
                $$\iff$$
                \begin{equation*}
                \begin{split}
                    L = \sqrt{2 + L}
                \end{split}
                \end{equation*}
                $$\iff$$
                \begin{equation*}
                \begin{split}
                    L^2 - L - 2 = 0
                \end{split}
                \end{equation*}
                $$\iff$$
                \begin{equation*}
                \begin{split}
                    L = 2 \mtext{or} L =-1.
                \end{split}
                \end{equation*}
            So it must be the case that $(x_n)_n \rightarrow L$.
        \end{proof}
%%%%%%%%%%%%%%%%%%%%%%%%%%%%%%%%%%%%%%%%%%%%%% 
    \begin{exercise}
        Does the following sequence converge?
            \begin{equation*}
            \begin{split}
                x_n := \sum_{k = n+1}^{2n} \frac{1}{k}.
            \end{split}
            \end{equation*}
    \end{exercise}
        \begin{proof}
            Claim: $x_n \leq 1$ for all $n$. Observe that:
                \begin{equation*}
                \begin{split}
                    x_n 
                    & = \sum_{k = n+1}^{2n} \frac{1}{k} \\
                    & = \frac{1}{n+1} + \frac{1}{n+2} + \frac{1}{n+3} + ... + \frac{1}{2n-2} + \frac{1}{2n-1} + \frac{1}{2n} \\
                    & \leq \frac{1}{n+1} + \frac{1}{n+1} + \frac{1}{n+1} + ... + \frac{1}{n+1} + \frac{1}{n+1} + \frac{1}{n+1} \\
                    & = \frac{n+1}{n+1} \\
                    & = 1.
                \end{split}
                \end{equation*}
            Claim: $x_{n} \leq x_{n+1}$. We have:
                \begin{equation*}
                \begin{split}
                    x_n \leq x_{n+1}
                    & \iff \sum_{k = n+1}^{2n} \frac{1}{k} \leq \sum_{k = n+2}^{2n+2}\frac{1}{k} \\
                    &\iff \frac{1}{n+1} \leq \frac{1}{2n+1} + \frac{1}{2n+1} \\
                    &\iff \frac{1}{n+1} \leq \frac{4n+3}{(2n+1)(2n+1)} \\
                    &\iff n+1  \geq \frac{4n^2 + 6n + 2}{4n+3}\\
                    &\iff 4n^2 + 7n +3 \geq 4n^2 + 6n + 2 \\
                    &\iff  7n + 3 \geq 6n + 2
                \end{split}
                \end{equation*}
            which is true for all $n \in \bfN$. Since $(x_n)_n$ is increasing and bounded above, by the monotone convergence theorem $(x_n)_n$ converges.
        \end{proof}
%%%%%%%%%%%%%%%%%%%%%%%%%%%%%%%%%%%%%%%%%%%%%%
    \begin{exercise}
        Let $(f_n)_n$ denote the Fibonacci sequence and let
            \begin{equation*}
            \begin{split}
                x_n := \frac{f_{n+1}}{f_n}.
            \end{split}
            \end{equation*}
        Given that $(x_n)_n$ converges, find its limit.
    \end{exercise}
        \begin{proof}
            Note that:
                \begin{equation*}
                \begin{split}
                    x_n 
                    &= \frac{f_{n+1}}{f_n} \\
                    &= \frac{f_{n} + f_{n-1}}{f_n} \\
                    &= 1 + \frac{f_{n-1}}{f_n} \\
                    & = 1 + \frac{1}{{f_n}/f_{n-1}} \\
                    & = 1 + \frac{1}{x_{n-1}}.
                \end{split}
                \end{equation*}
            If $(x_n)_n \rightarrow L$, then:
                \begin{equation*}
                \begin{split}
                    L = 1 + \frac{1}{L}
                    &\iff L^2 = L + 1 \\
                    &\iff L^2 - L - 1 = 0 \\
                    &\iff L = \frac{1 \pm \sqrt{5}}{2}.
                \end{split}
                \end{equation*}
            Since $\frac{1 - \sqrt{5}}{2} < 0$, it must be the case that $(x_n)_n \rightarrow \frac{1 + \sqrt{5}}{2}$
        \end{proof}
%%%%%%%%%%%%%%%%%%%%%%%%%%%%%%%%%%%%%%%%%%%%%%
    \begin{exercise}
        If $(x_n)_n$ is an unbounded sequence of reals numbers, show that there is a subsequence $(x_{n_k})_k$ such that:
            \begin{equation*}
            \begin{split}
                \left(\frac{1}{x_{n_k}}\right)_k \rightarrow 0.
            \end{split}
            \end{equation*}
    \end{exercise}
        \begin{proof}
            Since $(x_n)_n$ is an unbounded real sequence:
                \begin{equation*}
                \begin{split}
                    (\exists \epsilon_0 > 0)(\forall N \in \bfN) \ni (\exists n \in \bfN)(n \geq N \hspace{4pt}\land\hspace{4pt}|x_n - 0| \geq \epsilon_0).
                \end{split}
                \end{equation*}
            We can construct a subsequence as follows:
                \begin{equation*}
                \begin{split}
                    N = 1 &\implies (\exists n_1 \in \bfN)(n_1 \geq 1 \hspace{4pt}\land\hspace{4pt} |x_{n_1}| \geq \epsilon_0)\\
                    N = n_1 = 1 & \implies (\exists n_2 \in \bfN)(n_2 \geq n_1 \hspace{4pt}\land\hspace{4pt} |x_{n_2}| \geq \epsilon_0)\\
                    &\vdots
                \end{split}
                \end{equation*}
            Inductively, we obtain a sequence $(x_{n_k})_k$ which properly diverges to $+\infty$. Given $\epsilon > 0$, let $K$ be arbitrarily big so that $\epsilon > \frac{1}{n_K}$. Then for $k \geq K$, we have $\left|\frac{1}{n_k}\right| < \epsilon$.
        \end{proof}
%%%%%%%%%%%%%%%%%%%%%%%%%%%%%%%%%%%%%%%%%%%%%%
    \begin{exercise}
        Suppose that every subsequence of a sequence $(x_n)_n$ has a subsequence that converges to $0$. Show that $(x_n)_n \rightarrow 0$.
    \end{exercise}
        \begin{proof}
            Suppose towards contradiction that $(x_n)_n \not\rightarrow 0$. Then there exists a subsequence $(x_{n_k})_k \not\rightarrow 0$. By definition:
                \begin{equation*}
                \begin{split}
                    (\exists \epsilon_0 > 0)(\forall K \in \bfN) \ni (\exists k \in \bfN)(k \geq K \hspace{4pt}\land \hspace{4pt} d(x_{n_k} , 0) \geq \epsilon_0).
                \end{split}
                \end{equation*}
            We will construct a subsequence of $(x_{n_k})_k$ as follows:
                \begin{equation*}
                \begin{split}
                    K = 1 &\implies (\exists k_1 \in \bfN)(k_1 \geq 1 \hspace{4pt}\land\hspace{4pt} d(x_{n_{k_1}}, 0) \geq \epsilon_0) \\
                    K = k_1 + 1 &\implies (\exists k_2 \in \bfN)(k_2 \geq k_1 \hspace{4pt}\land\hspace{4pt} d(x_{n_{k_2}}, 0) \geq \epsilon_0) \\
                    &\vdots 
                \end{split}
                \end{equation*}
            Inductively, we obtain a sequence $(x_{n_{k_j}})_j \not\rightarrow 0$. But this contradicts our claim that every subsequence has a subsequence which converges to $0$. Hence it must be that $(x_n)_n \rightarrow 0$.
        \end{proof}
%%%%%%%%%%%%%%%%%%%%%%%%%%%%%%%%%%%%%%%%%%%%%%
    \begin{exercise}
        Let $(I_n)_n$ be a nested sequence of closed and bounded intervals. For each $n \in \bfN$ let $x_n \in I_n$. Use the Bolzano-Weierstrass Theorem for the sequence $(x_n)_n$ to give a proof of the Nested Intervals Property, that is to show that
            \begin{equation*}
            \begin{split}
                \bigcap_{n \geq 1}I_n \neq \emptyset.
            \end{split}
            \end{equation*}
    \end{exercise}
        \begin{proof}
            For each $n \in \bfN$, let $x_n \in I_n$. Then $(x_n)_n$ is bounded. By the Bolzano-Weirstrass theorem, $(x_n)_n$ admits a convergent subsequence $(x_{n_k})_k \rightarrow x$. Given $\epsilon > 0$, there exists a natural number $N$ such that $n_k \geq k \geq N$ implies $x_{n_k} \in V_\epsilon(x)$. Moreover, for $n = n_k$, we have $V_\epsilon(x) \subseteq I_n$, implying that $x\in I_n \subseteq I_{n-1} \subseteq ...$ Thus $x \in \bigcap_{n\geq 1}I_n$, establishing that the intersection is nonempty.
        \end{proof}
%%%%%%%%%%%%%%%%%%%%%%%%%%%%%%%%%%%%%%%%%%%%%%
    \begin{exercise}
        If $(x_n)_n$ is a bounded sequence and $s:=\sup_n x_n$ is such that $s \not\in \{x_n | n\geq 1\}$, show that there is a subsequence $(x_{n_k})_k$ that converges to $s$.
    \end{exercise}
        \begin{proof}
            Using the supremum property, we will construct a subsequence as follows:
                \begin{equation*}
                \begin{split}
                   k = 1 &\implies \exists n_1 \ni  s-1 < x_{n_1} < u \\                  
                \end{split}
                \end{equation*}
            Because $(s-1,s)\cap \{x_n \mid n \in \bfN\}$ is infinite, we have:
                \begin{equation*}
                \begin{split}
                   k = 2 &\implies \exists n_2 \ni  s-\frac{1}{2} < x_{n_2} < u \\
                   &\vdots
                \end{split}
                \end{equation*}
            Inductively, we obtain $s - \frac{1}{k} < x_{n_k} < s$. By the squeeze theorem, $(x_{n_k}) \rightarrow s$. 
        \end{proof}
%%%%%%%%%%%%%%%%%%%%%%%%%%%%%%%%%%%%%%%%%%%%%%
    \begin{exercise}
        Let $(x_n)_n$ and $(y_n)_n$ be bounded sequences. Show that
            \begin{equation*}
            \begin{split}
                \limsup((x_n + y_n)_n) \leq \limsup(x_n)_n + \limsup(y_n)_n
            \end{split}
            \end{equation*}
    \end{exercise}
        \begin{proof}
            We have $x_k + y_k \leq \sup_{m \geq n}x_m + \sup_{m \geq n}y_n$ for $k \geq n$. This implies that $\sup_{m \geq n}x_m + \sup_{m \geq  n}y_n$ is an upperbound of $x_k + y_k$. Whence $\sup_{k \geq n}(x_k + y_k) \leq \sup_{m \geq n}x_m + \sup_{m \geq  n}y_n$. Taking the limit of both sides gives $\limsup (x_n + y_n) \leq \limsup x_n + \limsup y_n$.
        \end{proof}
%%%%%%%%%%%%%%%%%%%%%%%%%%%%%%%%%%%%%%%%%%%%%%
    \begin{exercise}
        Let $(x_n)_n$ be a bounded sequence. Show that:
            \begin{equation*}
            \begin{split}
                \liminf(x_n)_n = \sup\{t \in \bfR \mid \{n \mid x_n < t \} \hspace{-2pt}\mtext{is finite}\hspace{-2pt}\}.
            \end{split}
            \end{equation*}
    \end{exercise}
        \begin{proof}
            Let $l = \liminf(x_n)_n = \sup_{m \geq 1}(\inf_{n \geq m}x_n)$. By the supremum property, we have $l - \epsilon < (\inf_{n \geq m} x_n)_n \leq l$. So given any $M \in \bfN$, there are only finitely many $x_n$ with $x_n < \inf_{m \geq M}$, hence $\{n \mid x_n < l - \epsilon\}$ is finite. Setting $t = l - \epsilon$ gives $l = \sup\{t \in \bfR \mid \{n \mid x_n < t \} \hspace{-2pt}\mtext{is finite}\hspace{-2pt}\}$.
        \end{proof}
%%%%%%%%%%%%%%%%%%%%%%%%%%%%%%%%%%%%%%%%%%%%%%
    \begin{exercise}
        Let $(x_n)_n$ be a bounded sequence. Show that
            \begin{equation*}
            \begin{split}
                \liminf(-x_n)_n = -\limsup(x_n)_n.
            \end{split}
            \end{equation*}
    \end{exercise}
        \begin{proof}
            We have:
                \begin{equation*}
                \begin{split}
                    -\limsup x_n 
                    & = -\inf_{m\geq 1}(\sup_{n \geq m}x_n) \\
                    & = \sup_{m \geq 1}(-\sup_{n \geq m}x_n) \\
                    & = \sup_{m \geq 1}(\inf_{n \geq m}-x_n) \\
                    & = \liminf -x_n.
                \end{split}
                \end{equation*}
        \end{proof}
%%%%%%%%%%%%%%%%%%%%%%%%%%%%%%%%%%%%%%%%%%%%%%
\end{document}

