%%%%%%%PACKAGES%%%%%%%
\documentclass[10pt,twoside,openany]{memoir}


\usepackage[math]{anttor}
\usepackage[T1]{fontenc}


\usepackage{titlesec}
    \titlespacing*{\chapter}
    {0pt} % Left margin
    {*1} % Space before the chapter number (increase this value for more space)
    {0pt} % Space after the chapter number and before the title
\usepackage{anyfontsize}
\usepackage{fancybox}
\usepackage[dvipsnames,svgnames,x11names,hyperref]{xcolor}
\usepackage{enumerate}
\usepackage{comment}
\usepackage{amsfonts}
\usepackage{amsthm}
\usepackage{amsmath}
\usepackage{amssymb}
\usepackage{mathrsfs}
\usepackage{hyperref}
\usepackage{fullpage}
\usepackage{bm}
\usepackage{cprotect}
\usepackage{calligra}
\usepackage{emptypage}
\usepackage{titleps}
\usepackage{microtype}
\usepackage{float}
\usepackage{ocgx}
\usepackage{appendix}
\usepackage{graphicx}
\usepackage{pdfcomment}
\usepackage{enumitem}
\usepackage{mathtools}
\usepackage{tikz-cd}
\usepackage{relsize}
\usepackage[font=footnotesize,labelfont=bf]{caption}
\usepackage{changepage}
\usepackage{xcolor}
\usepackage{ulem}
\usepackage{pgfplots}
\usepackage{marginnote}
    \newcommand*{\mnote}[1]{ % <----------
    \checkoddpage
    \ifoddpage
        \marginparmargin{left}
    \else
        \marginparmargin{right}
    \fi
        \marginnote{\tiny \textcolor{oorange}{#1}}
    }
\usepackage{datetime}
    \newdateformat{specialdate}{\THEYEAR\ \monthname\ \THEDAY}
\usepackage[margin=0.9in]{geometry}
    \setlength{\voffset}{-0.4in}
    \setlength{\headsep}{30pt}
\usepackage{fancyhdr}
    \fancyhf{}
    \cfoot{\footnotesize \thepage}
    \fancyhead[R]{\footnotesize \rightmark}
    \fancyhead[L]{\footnotesize \leftmark}
\usepackage[outline]{contour}% http://ctan.org/pkg/contour
    \renewcommand{\arraystretch}{1.5}
    \contourlength{0.4pt}
    \contournumber{10}%
\usepackage{letterspace}
    \linespread{1.25}
\usepackage{thmtools}
    \declaretheoremstyle[
        spaceabove=6pt, spacebelow=6pt,
        headfont=\normalfont\bfseries,
        notefont=\mdseries, notebraces={(}{)},
        bodyfont=\normalfont,
        postheadspace=1em
        %qed=\qedsymbol
        ]{mystyle}

    \declaretheorem[
        numberwithin=section,
        %shaded={
        %    rulecolor={RGB}{255,250,177},
        %    rulewidth=5pt, 
        %    bgcolor={RGB}{255,250,177}}
    ]{theorem}

    \declaretheorem[
        sibling=theorem,
        numberwithin=section,
        %shaded={
        %    rulecolor=Lavender,
        %    rulewidth=5pt, 
        %    bgcolor=Lavender}
    ]{lemma}

    \declaretheorem[
        sibling=theorem,
        numberwithin=section,
        %shaded={
        %    rulecolor=Lavender,
        %    rulewidth=5pt, 
        %    bgcolor=Lavender}
    ]{proposition}

    \declaretheorem[
        sibling=theorem,
        numberwithin=section,
        %shaded={
        %    rulecolor=Lavender,
        %    rulewidth=5pt, 
        %    bgcolor=Lavender}
    ]{corollary}

    \declaretheorem[
        numberwithin=section,
        style=mystyle,
        %shaded={
        %    rulecolor={RGB}{233,233,233},
        %    rulewidth=5pt, 
        %    bgcolor={RGB}{233,233,233}}
    ]{example}

    \declaretheorem[
        numberwithin=section,
        style=mystyle,
        %shaded={
        %    rulecolor={RGB}{255,250,177},
        %    rulewidth=5pt, 
        %    bgcolor={RGB}{255,250,177}}
    ]{definition}

    \declaretheorem[
        %shaded={
        %    rulecolor=Lavender,
        %    rulewidth=5pt, 
        %    bgcolor=Lavender}
    ]{exercise}
\declaretheorem[numbered=unless unique,style=mystyle]{Note}
    




%%%%%%%%%%%%%%%%%%%%%%
%%%%%%%%MACROS%%%%%%%%
%%%%%%%%%%%%%%%%%%%%%%
\input{/Users/gcrescenzo/Documents/School/LaTeX Documents/Class Notes/makros.tex}




%%%%%%%%%%%%%%%%%%%%%%
%%%%DOCUMENT SETUP%%%%
%%%%%%%%%%%%%%%%%%%%%%
\setsecnumdepth{subsection}
\definecolor{darkgreen}{rgb}{0, 0.5976, 0}
\hypersetup{pdfauthor=Gianluca Crescenzo, pdftitle=Real Analysis I Notes, pdfstartview=FitH, colorlinks=true, linkcolor=darkgreen, citecolor=darkgreen}


%This adds a "front cover" page.
%{\thispagestyle{empty}
%\vspace*{\fill}
%\begin{tabular}{l}
%\begin{tabular}{l}
%\includegraphics[scale=0.24]{oxy-logo.png}
%\end{tabular} \\
%\begin{tabular}{l}
%\Large \color{black} Module Theory, Linear Algebra, and Homological Algebra \\ \Large \color{black} Gianluca Crescenzo
%\end{tabular}
%\end{tabular}
\begin{document}
\begin{center}
    { \Large Math 310 \\[0.1in]Homework 3 \\[0.1in]
    Due: 9/27/2024}\\[.25in]
    { Name:} {\underline{Gianluca Crescenzo\hspace*{2in}}}\\[0.15in]
    \end{center}
    \vspace{4pt}
%%%%%%%%%%%%%%%%%%%%%%%%%%%%%%%%%%%%%%%%%%%%%%%%%%%%%%%%%%%%%%%%%%%%%%%%%%%%%%%%%%%%%%%%%%%%%%%%%%%%%%%%%%%%%%%   
    \begin{exercise}
        Find $\Sup{(A)}$ and $\Inf{(A)}$ where:
            \begin{enumerate}[label = (\arabic*)]
                \item $A_1 = \left\{1 - \frac{(-1)^n}{n} \mid n \in \bfN\right\}$.
                \item $A_2 = \left\{\frac{1}{n} - \frac{1}{m} \mid m,n \in \bfN\right\}$.
                \item $A_3 = \left\{ \frac{m}{n} \mid m,n \in \bfN,\hspace{2pt} m+n \leq 10\right\}$.
            \end{enumerate} 
    \end{exercise}
        {\color{red} \begin{proof}
            Claim: $\Inf{(A_1)} = \frac{1}{2}$. Note that $\frac{1}{2}$ is a lowerbound because $\frac{1}{2} \leq a$ for all $a \in A_1$. Let $t$ be a lowerbound of $A_1$. If $t \leq \frac{1}{2}$, then we are done. If $t>\frac{1}{2}$, then $t - \frac{1}{2} > 0$. By the Archimedean Property, there exists an element $n \in \bfN$ with $t - \frac{1}{2} > \frac{1}{n}$ This gives $t > \frac{1}{2} + \frac{1}{n}$, which is a contradiction because $\frac{1}{2}+\frac{1}{n} \in A_1$ for all positive natural numbers. Thus $\inf{(A_1)} = \frac{1}{2}$. Note that $2 \geq 1  + \left|  - \frac{(-1)^n}{n}\right| = 1 + \frac{(-1)^n}{n}$ for all $n \in \bfN$. Hence $2$ is an upper bound. Furthermore, since $2 \in A_1$, it must be the case that $\sup(A_1) = 2$.

            (2) 

            (3) Note that $\frac{1}{9} \leq \frac{m}{n} \leq \frac{9}{1}$ for all $m,n \in \bfN$, $m+n \leq 10$. So $\frac{1}{9}$ is a lower bound of $A_3$ and $\frac{9}{1}$ is an upper bound of $A_3$. Since $\frac{1}{9}, \frac{9}{1} \in A_3$, it must be the case that $\inf(A_3) = \frac{1}{9}$ and $\sup{(A_3)} = \frac{9}{1}$.


        \end{proof}}
%%%%%%%%%%%%%%%%%%%%%%%%%%%%%%%%%%%%%%%%  
    \begin{exercise}
        Suppose $u = \Sup{(A)}$ such that $u \not\in A$. Show that there is a strictly increasing sequence
            \begin{equation*}
            \begin{split}
                t_1 < t_2 < t_3 < ...
            \end{split}
            \end{equation*}
        with $t_n \in A$ and $t_n + \frac{1}{n} > u$ for all $n \geq 1$.
    \end{exercise}  
        {\color{red} \begin{proof}
            Note that for all $\epsilon > 0$, there exists an $a_\epsilon$ with $u - \epsilon < a_\epsilon$. Define:
                \begin{equation*}
                \begin{split}
                    t_1 &> u - 1 \\
                    t_2 &> \max \left\{t_1, u - \frac{1}{2}\right\} \\
                    t_3 &> \max \left\{t_2, u - \frac{1}{3}\right\} \\
                    &\vdots \\
                    t_n &> \max \left\{t_{n-1}, u - \frac{1}{n} \right\}.
                \end{split}
                \end{equation*}
            If $\max \left\{t_{n-1}, u - \frac{1}{n} \right\} = t_{n-1}$, then clearly $t_n > t_{n-1}$. If $\max \left\{t_{n-1}, u - \frac{1}{n} \right\} = u - \frac{1}{n}$, then $t_n > u - \frac{1}{n} > t_{n-1}$. This gives $t_n + \frac{1}{n} > u$ for all $n \geq 1$, and furthermore, we obtain a strictly increasing sequence:
                \begin{equation*}
                \begin{split}
                    t_1 < t_2 < t_3 < ... 
                \end{split}
                \end{equation*}
                \qedhere
        \end{proof}}
%%%%%%%%%%%%%%%%%%%%%%%%%%%%%%%%%%%%%%%%  
    \begin{exercise}
        If $m$ is a lower bound for $A \subseteq \bfR$, show that the following are equivalent:
            \begin{enumerate}[label = (\arabic*)]
                \item $m = \inf{(A)}$.
                \item For all $t>m$, there exists $a_t \in A$ with $a_t <  t$.
                \item For all $\epsilon > 0$ there exists $a_\epsilon \in A$ with $m+\epsilon > a_\epsilon$.
            \end{enumerate}
    \end{exercise}
        {\color{red} \begin{proof}
            Let $m = \Inf{(A)}$. Assuming $t > m$, suppose towards contradiction there does not exist an $a \in A$ with $a < t$. Then it must be the case that $m < t \leq a$ for all $t > m$. This is a contradiction, because $m$ is the greatest lower bound.

            Now assume for all $t > m$, there exists $a_t \in A$ with $a_t < t$. Given $\epsilon > 0$, pick $t = m + \epsilon$. Then by (2) there exists an $a_t$ with $m+ \epsilon > a_t$.

            Now assume for all $\epsilon >0$ there exists $a_\epsilon \in A$ with $m + \epsilon > a_\epsilon$. Given that $m$ is a lower bound for $A$, assume there exists another lower bound for $A$ with $l > m$. Pick $\epsilon = l - m$, then there exists an $a \in A$ with $m + (l - m) > a$. Simplifying yields $l > a$, which contradicts $l$ being a lower bound. Hence $\inf{(A)} = m$.
        \end{proof}}
%%%%%%%%%%%%%%%%%%%%%%%%%%%%%%%%%%%%%%%%  
    \begin{exercise}
        Let $A,B \subseteq \bfR$ be bounded subsets.
            \begin{enumerate}[label = (\arabic*)]
                \item Show that
                    \begin{equation*}
                    \begin{split}
                        \Sup{(A+B)} &= \Sup{(A)} + \Sup{(B)}, \\
                        \Inf(A+B) &= \Inf(A) + \Inf(B).
                    \end{split}
                    \end{equation*}
                \item If $t>0$, show that 
                    \begin{equation*}
                    \begin{split}
                        \Sup(tA) &= t \Sup(A), \\
                        \Inf(tA) &= t \Inf(A).
                    \end{split}
                    \end{equation*}
            \end{enumerate}
                {\color{red} \begin{proof}
                    (1) Define $\Sup{(A)} = u$ and $\Sup{(B)} = v$. Then for all $\epsilon > 0$, there exists $a_\epsilon \in A$, $b_\epsilon \in B$ with $u - \epsilon < a_\epsilon$ and $v - \epsilon < b_\epsilon$. Pick $\epsilon = \frac{\epsilon}{2}$. Then adding both inequalities gives $(u + v) - \epsilon < a_\epsilon + b_\epsilon \in A+B$. Hence $\Sup(A+B) = u + v = \Sup(A) + \Sup(B)$. Similarly, define $\Inf(A) = m$ and $\Inf(B) = n$. Then for all $\epsilon > 0$, there exists $a_\epsilon \in A$, $b_\epsilon \in B$ with $m + \epsilon > a_\epsilon$ and $n + \epsilon > b_\epsilon$. Pick $\epsilon = \frac{\epsilon}{2}$. Then adding both inequalities gives $(m+n)+\epsilon > a_\epsilon + b_\epsilon \in A+B$. Hence $\Inf(A+B) = m + n = \Inf(A) + \Inf(B)$.

                    (2) Let $\sup(A) = u$. Then $a \leq u $ for all $a \in A$. We have that $u - \epsilon < a$ for some $a \in A$. Pick $\epsilon = \frac{\epsilon}{t}$. Then $t u - \epsilon < ta$ for some $t a \in tA$. Hence $\sup(tA) = tu = t\sup(A)$. Similarly, let $\inf(A) = m$. Then $m \leq a$ for all $a \in A$. We have that $m+\epsilon > a$ for some $a \in A$. Pick $\epsilon = \frac{\epsilon}{t}$. Then $tm + \epsilon > ta$ for some $ta \in tA$. Hence $\inf(tA) = tm = t\inf(A)$.
                \end{proof}}
    \end{exercise}
%%%%%%%%%%%%%%%%%%%%%%%%%%%%%%%%%%%%%%%%  
    \begin{exercise}
        Let $I = (0,1)$ denote the open interval and consider the function
            \begin{equation*}
            \begin{split}
                F:I \times I \rightarrow \bfR \mtext{defined by} F(x,y) = 2x + y.
            \end{split}
            \end{equation*}
        Compute
            \begin{equation*}
            \begin{split}
                \sup_{y \in I} \left(\inf_{x \in I} F(x,y)\right),
            \end{split}
            \end{equation*}
        and
            \begin{equation*}
            \begin{split}
                \inf_{y \in I} \left(\sup_{x \in I} F(x,y)\right).
            \end{split}
            \end{equation*}
        Are they equal?
    \end{exercise}
        {\color{red} \begin{proof}
            Observe that:
                \begin{equation*}
                \begin{split}
                    \sup_{y \in I}\left(\inf_{x \in I}(2x+y)\right)
                    & = \sup_{y \in I}\left(2\inf_{x \in I}x+\inf_{x \in I}y\right) \\
                    & = \sup_{y \in I}y \\
                    & = 1,
                \end{split}
                \end{equation*}
                \begin{equation*}
                \begin{split}
                    \inf_{y \in I}\left(\sup_{x \in I}(2x+y)\right)
                    & = \inf_{y \in I} \left( \sup_{x \in I}2x + \sup_{x \in I}y\right) \\
                    & = \inf_{y \in I} \left( 2 + y\right) \\
                    & = \inf_{y \in I}2 + \inf_{y \in I}y \\
                    & = 2.
                \end{split}
                \end{equation*}
        \end{proof}}
%%%%%%%%%%%%%%%%%%%%%%%%%%%%%%%%%%%%%%%%
    \begin{exercise}
        Let $D$ be a nonempty set and consider the set of all bounded functions:
            \begin{equation*}
            \begin{split}
                \ell_\infty(D) := \{f \mid f:D \rightarrow \bfR \hspace{4pt}\text{is bounded}\}
            \end{split}
            \end{equation*}
        with point-wise addition and scalar multiplication. Show that
            \begin{equation*}
            \begin{split}
                d_u(f,g) := \sup_{x \in D}\left|f(x) - g(x)\right|
            \end{split}
            \end{equation*}
        defines a metric on $\ell_\infty(D)$. We call $d_u$ the \textbf{uniform metric}.
    \end{exercise}
        {\color{red} \begin{proof}
            Observe that:
                \begin{equation*}
                \begin{split}
                    d_u(f,g)
                    & = \sup_{x \in D}\left(\left|f(x) - g(x)\right|\right) \\
                    & = \sup_{x \in D}\left(\left|g(x) - f(x)\right|\right) \\
                    & = d_u(g,f).
                \end{split}
                \end{equation*}
            Thus $(\ell_\infty,d_u)$ is symmetric. We also have that:
                \begin{equation*}
                \begin{split}
                    d_u(f,h)
                    & = \sup_{x \in D}\left(\left|f(x) - h(x)\right|\right) \\
                    & = \sup_{x \in D}\left(\left|f(x) - g(x) + g(x) - h(x)\right|\right)\\
                    & \leq \sup_{x \in D}\left(\left|f(x)-g(x)\right| + \left|g(x) - h(x)\right|\right)\\
                    & = \sup_{x \in D}\left(\left|f(x)-g(x)\right|\right) + \sup_{x \in D}\left(\left|g(x)-h(x)\right|\right)\\
                    & = d(f,g) + d(g,h).
                \end{split}
                \end{equation*}
            Hence $(\ell_\infty,d_u)$ satisfies the triangle-inequality. Furthermore:
                \begin{equation*}
                \begin{split}
                    d_u(f,f)
                    & = \sup_{x \in D}\left(\left|f(x) - f(x)\right|\right) \\
                    & = \sup_{x \in D}0 \\
                    & = 0.
                \end{split}
                \end{equation*}
            Lastly $d_u(f,g)=0$ implies $\sup_{x \in D}\left(\left|f(x) - g(x)\right|\right) = 0$. By definition of the absolute value, $|f(x)-g(x)| \geq 0$, so it must be the case that $|f(x)-g(x)| = 0$. Hence $f(x) = g(x)$, establishing that $(\ell_\infty,d_u)$ forms a metric space.
        \end{proof}}
%%%%%%%%%%%%%%%%%%%%%%%%%%%%%%%%%%%%%%%%
    \begin{exercise}
        Let $f,g:D \rightarrow \bfR$ be bounded functions. Show that
            \begin{enumerate}[label = (\arabic*)]
                \item $\sup_{x\in D}(f+g)(x) \leq \sup_{x\in D}f(x) + \sup_{x\in D}g(x)$.
                \item $\inf_{x\in D}(f+g)(x) \leq \inf_{x\in D}f(x) + \inf_{x\in D}g(x)$.
                \item $\left|\sup_{x \in D}f(x) - \sup_{x \in D}g(x)\right| \leq \sup_{x\in D}\left|f(x) - g(x)\right|$.
            \end{enumerate}
    \end{exercise}
%%%%%%%%%%%%%%%%%%%%%%%%%%%%%%%%%%%%%%%%
    \begin{exercise}
        Find $\bigcap_{n = 1}^\infty I_n$ where
            \begin{enumerate}[label = (\arabic*)]
                \item $I_n = \left[0,\frac{1}{n}\right]$,
                \item $I_n = \left(0, \frac{1}{n}\right)$,
                \item $I_n = \left[n , \infty\right)$.
            \end{enumerate}
    \end{exercise}
        {\color{red} \begin{proof}
            (1) Note that $[0,\frac{1}{n}]$ is closed and bounded for all $n \geq 1$. Note that:
                \begin{equation*}
                \begin{split}
                    \inf \{\text{length}\left(\left[0,1/n\right]\right) \mid n \geq 1 \} 
                     &= \inf_{n \geq 1} \left(\frac{1}{n} - 0\right) 
                      = 0.
                \end{split}
                \end{equation*}
            By the Nested Interval Theorem:
                \begin{equation*}
                \begin{split}
                    \bigcap_{n=1}^\infty \left[0 , \frac{1}{n}\right] = \sup_{n \geq 1} 0 = \inf_{n \geq 1} \frac{1}{n} = 0.
                \end{split}
                \end{equation*}

            (2) Claim: $\bigcap_{n=1}^\infty \left(0, \frac{1}{n}\right) = \emptyset$. Suppose towards contradiction there exists $t \in \bigcap_{n=1}^\infty \left(0, \frac{1}{n}\right)$. Then $t \in \left(0 ,\frac{1}{n}\right)$ for all $n \geq 1$. So $t < \frac{1}{n}$ implies $\frac{1}{t} > n$ for all $n\geq 1$, meaning $\bfN$ is bounded above. This is a contradiction, hence $\bigcap_{n=1}^\infty \left(0, \frac{1}{n}\right) = \emptyset$.

            (3) Claim: $\bigcap_{n=1}^\infty \left[n, \infty\right) = \emptyset$. Suppose towards contradiction there exists $t \in \bigcap_{n=1}^\infty \left[n, \infty\right)$. Then $t \in [n,\infty)$ for all $n \geq 1$. So $t \geq n$ for all $n \geq 1$. Hence $\bfN$ is bounded above, which is a contradiction. Thus $\bigcap_{n=1}^\infty \left[n, \infty\right) = \emptyset$.
        \end{proof}}
%%%%%%%%%%%%%%%%%%%%%%%%%%%%%%%%%%%%%%%%
    \begin{exercise}
        If $x>0$, show that there is an $n \in \bfN$ with $\frac{1}{2^n} <x$.
    \end{exercise}
        {\color{red} \begin{proof}
            By the Archimedean Property 2, there exists $n \in \bfN$ such that $0 < \frac{1}{n} < x$. Claim: $\frac{1}{2^n} < \frac{1}{n}$. It suffices to show that $2^n > n$. Bernoulli's inequality gives $(1+1)^n \geq 1 + n$, hence $2^n > n$.
        \end{proof}}
%%%%%%%%%%%%%%%%%%%%%%%%%%%%%%%%%%%%%%%%
    \begin{exercise}
        The \textbf{Dyadic Rationals} are defined as 
            \begin{equation*}
            \begin{split}
                \bfD := \left\{\frac{m}{2^n} \mid m,n \in \bfZ\right\}.
            \end{split}
            \end{equation*}
        Show that $\bfD \subseteq \bfR$ is dense.
    \end{exercise}
        {\color{red} \begin{proof}
            Let $I = (a,b)$. Then $b-a > 0$. By Archimedean Property 2 there exists $n \in \bfN$ such that $b-a > \frac{1}{n}$. Exercise 9 gives that $b - a > \frac{1}{2^n}$ for some $n \in \bfZ$. This simplifies to $2^nb > 1 + 2^na$. Since $2^na \in \bfR$, there exists $m \in \bfZ$ with $m-1 \leq 2^na < m$, implying that $a < \frac{m}{2^n}$. Furthermore, we also have that $m \leq 1 + 2^n a < m+1$, and substituting for $2^n b$ gives $m < 2^n b$. So $\frac{m}{2^n} < b$, which means $\frac{m}{2^n} \in (a,b)$. Thus $I \cap D \neq \emptyset$.
        \end{proof}}
\end{document}
